Strip block fs to just managing journal kinds

src/Dafny/examples/fs/fs.dfy
@@ -20,31 +20,6 @@ module Fs {
 
   datatype Option<T> = Some(x:T) | None
 
-  datatype preInodeData = InodeData(sz: nat, blks: seq<Block>)
-  {
-    static const preZero: preInodeData := InodeData(0, C.repeat(block0, 15))
-    static const zero: InodeData := preZero
-
-    const num_used: nat := Round.div_roundup_alt(sz, 4096)
-
-    predicate Valid()
-    {
-      && |blks| == 15
-      && sz <= Inode.MAX_SZ
-    }
-
-    static lemma zero_valid()
-      ensures zero.Valid()
-    {}
-
-    function used_blocks(): seq<Block>
-      requires Valid()
-    {
-      blks[..num_used]
-    }
-  }
-  type InodeData = d:preInodeData | d.Valid() witness preInodeData.preZero
-
   function zero_lookup(m: map<Blkno, Block>, bn: Blkno): Block
     requires blkno_dom(m)
     requires blkno_ok(bn)
@@ -64,17 +39,8 @@ module Fs {
     forall ino: Ino :: ino_ok(ino) <==> ino in m
   }
 
-  predicate Valid_inode_blks(inode_blks: map<Ino, InodeData>)
-    requires ino_dom(inode_blks)
+  class Filesys<AllocState>
   {
-    forall ino | ino_ok(ino) :: inode_blks[ino].Valid()
-  }
-
-  class Filesys
-  {
-
-    // block-based inodes
-    ghost var inode_blks: map<Ino, InodeData>;
 
     // inodes, block_used, and data_block are basically just the data in the
     // journal (except block_used additionally has inode owners)
@@ -82,8 +48,8 @@ module Fs {
     // encoded inodes on disk
     ghost var inodes: map<Ino, Inode.Inode>;
     ghost var cur_inode: Option<(Ino, Inode.Inode)>;
-    // allocator state + the inode that owns the block
-    ghost var block_used: map<Blkno, Option<Ino>>;
+    // allocator state + some stuff
+    ghost var block_used: map<Blkno, Option<AllocState>>;
     // on-disk value for all the data blocks
     ghost var data_block: map<Blkno, Block>;
 
@@ -103,10 +69,9 @@ module Fs {
       && blkno_dom(block_used)
       && blkno_dom(data_block)
       && ino_dom(inodes)
-      && ino_dom(inode_blks)
     }
 
-    predicate {:opaque} Valid_jrnl_to_block_used(block_used: map<Blkno, Option<Ino>>)
+    predicate {:opaque} Valid_jrnl_to_block_used(block_used: map<Blkno, Option<AllocState>>)
       reads jrnl
       requires blkno_dom(block_used)
       requires Valid_basics(jrnl)
@@ -157,54 +122,11 @@ module Fs {
       forall ino: Ino | ino in inodes :: inodes[ino].Valid()
     }
 
-    static predicate {:opaque} Valid_inodes_to_block_used(inodes: map<Ino, Inode.Inode>, block_used: map<Blkno, Option<Ino>>)
-      requires blkno_dom(block_used)
-    {
-      && (forall ino: Ino | ino in inodes ::
-        && (forall bn | bn in inodes[ino].blks ::
-          bn != 0 ==>
-          && blkno_ok(bn)
-          && block_used[bn] == Some(ino))
-        )
-    }
-
     predicate Valid_inodes()
       requires Valid_domains()
       reads this
     {
       && Inodes_all_Valid(inodes)
-      && Valid_inodes_to_block_used(inodes, block_used)
-    }
-
-    static predicate {:opaque} blks_match?(blk_offs: seq<Blkno>, blks: seq<Block>, data_block: map<Blkno, Block>)
-      requires |blk_offs| == |blks|
-      requires blkno_dom(data_block)
-    {
-      forall k: nat | k < |blk_offs| ::
-        && blkno_ok(blk_offs[k])
-        && blks[k] == zero_lookup(data_block, blk_offs[k])
-    }
-
-    // inode i encodes blks, using data_block to lookup indirect references
-    static predicate inode_blks_match(i: Inode.Inode, d: InodeData, data_block: map<Blkno, Block>)
-    {
-      && i.sz as nat == d.sz
-      && |d.blks| == |i.blks|
-      && d.Valid()
-      && blkno_dom(data_block)
-      && blks_match?(i.blks, d.blks, data_block)
-    }
-
-    static predicate Valid_inode_blks_match(
-      inodes: map<Ino, Inode.Inode>,
-      inode_blks: map<Ino, InodeData>,
-      data_block: map<Blkno, Block>)
-      requires ino_dom(inodes)
-      requires ino_dom(inode_blks)
-      requires blkno_dom(data_block)
-    {
-      && (forall ino: Ino | ino_ok(ino) ::
-         && inode_blks_match(inodes[ino], inode_blks[ino], data_block))
     }
 
     static const ballocMax: uint64 := super.data_bitmaps as uint64 * 4096*8 - 8
@@ -226,22 +148,6 @@ module Fs {
       && Valid_jrnl_to_inodes(inodes)
     }
 
-    predicate Valid_data()
-      reads this
-      requires Valid_domains()
-    {
-      && Valid_inode_blks_match(inodes, inode_blks, data_block)
-    }
-
-    lemma inode_blks_sz(ino: Ino)
-      requires Valid_domains()
-      requires Valid_data()
-      requires ino_ok(ino)
-      ensures inodes[ino].sz as nat == inode_blks[ino].sz
-    {
-      assert inode_blks_match(inodes[ino], inode_blks[ino], data_block);
-    }
-
     function Repr(): set<object>
     {
       {this, jrnl} + balloc.Repr()
@@ -258,7 +164,6 @@ module Fs {
       && Valid_data_block(data_block)
       && Valid_jrnl_to_all()
       && this.Valid_inodes()
-      && this.Valid_data()
 
       && this.Valid_balloc()
     }
@@ -270,15 +175,12 @@ module Fs {
       && quiescent()
     }
 
-    lemma Valid_inode_data()
-      requires Valid_domains()
-      requires Valid_data()
-      ensures Valid_inode_blks(inode_blks)
-    {}
-
     constructor Init(d: Disk)
       ensures ValidQ()
-      ensures inode_blks == map ino | ino_ok(ino) :: InodeData.zero
+      ensures block_used == map bn: Blkno | blkno_ok(bn) :: None
+      ensures cur_inode == None
+      ensures inodes == map ino: Ino | ino_ok(ino) :: Inode.zero
+      ensures data_block == map bn: Blkno | blkno_ok(bn) :: block0
     {
       var jrnl := NewJrnl(d, fs_kinds);
       this.jrnl := jrnl;
@@ -287,22 +189,18 @@ module Fs {
 
       this.inodes := map ino: Ino | ino_ok(ino) :: Inode.zero;
       this.cur_inode := None;
-      this.inode_blks := map ino: Ino | ino_ok(ino) :: InodeData.zero;
       Inode.zero_encoding();
       this.block_used := map bn: uint64 | blkno_ok(bn) :: None;
       this.data_block := map bn: uint64 | blkno_ok(bn) :: block0;
       new;
-      InodeData.zero_valid();
-      jrnl.reveal_Valid();
-      reveal_Valid_inodes_to_block_used();
-      reveal_addrsForKinds();
+      reveal jrnl.Valid();
+      reveal addrsForKinds();
 
-      reveal_Valid_jrnl_to_block_used();
-      reveal_Valid_jrnl_to_data_block();
-      reveal_Valid_jrnl_to_inodes();
-      reveal_blks_match?();
-      reveal_DataBlk();
-      reveal_InodeAddr();
+      reveal Valid_jrnl_to_block_used();
+      reveal Valid_jrnl_to_data_block();
+      reveal Valid_jrnl_to_inodes();
+      reveal DataBlk();
+      reveal InodeAddr();
       assert Valid_inodes();
     }
 
@@ -376,58 +274,41 @@ module Fs {
       reveal_Valid_jrnl_to_block_used();
     }
 
-    lemma free_block_unused(bn: Blkno)
-      requires Valid()
-      requires bn != 0
-      requires blkno_ok(bn) && block_used[bn].None?
-      ensures forall ino | ino_ok(ino) :: bn !in inodes[ino].blks
+    // public
+    method getDataBlock(txn: Txn, bn: Blkno) returns (bs: Bytes)
+      modifies {}
+      requires Valid() ensures Valid()
+      requires this.jrnl == txn.jrnl
+      requires blkno_ok(bn)
+      ensures fresh(bs)
+      ensures is_block(bs.data)
+      ensures bs.data == zero_lookup(data_block, bn)
     {
-      reveal_Valid_inodes_to_block_used();
+      if bn == 0 {
+        bs := NewBytes(4096);
+        return;
+      }
+      datablk_inbounds(jrnl, bn);
+      bs := txn.Read(DataBlk(bn), 4096*8);
+      reveal_Valid_jrnl_to_data_block();
     }
 
     // public
-    method writeDataBlock(txn: Txn, bn: Blkno, blk: Bytes,
-      ghost ino: Ino, ghost blkoff: nat)
+    method writeDataBlock(txn: Txn, bn: Blkno, blk: Bytes)
       modifies this, jrnl
       requires Valid() ensures Valid()
       requires txn.jrnl == jrnl
       requires is_block(blk.data)
-      requires ino_ok(ino)
-      requires blkoff < |inode_blks[ino].blks|
-      requires inodes[ino].blks[blkoff] == bn
-      requires bn != 0
+      requires bn != 0 && blkno_ok(bn)
       ensures
       && inodes == old(inodes)
       && cur_inode == old(cur_inode)
       && block_used == old(block_used)
       && data_block == old(data_block)[bn := blk.data]
-      && inode_blks ==
-        old(var d0 := inode_blks[ino];
-            var d' := d0.(blks := d0.blks[blkoff:=blk.data]);
-            inode_blks[ino:=d'])
     {
-      assert inode_blks_match(inodes[ino], inode_blks[ino], data_block);
-      reveal_blks_match?();
       datablk_inbounds(jrnl, bn);
       txn.Write(DataBlk(bn), blk);
       data_block := data_block[bn := blk.data];
-      ghost var d0 := inode_blks[ino];
-      ghost var d' := d0.(blks := d0.blks[blkoff:=blk.data]);
-      inode_blks := inode_blks[ino:=d'];
-
-      ghost var i := inodes[ino];
-      inode_blks_match_change_1(i, d0, old(data_block), i, bn, blkoff, blk.data);
-
-      Filesys.reveal_Valid_inodes_to_block_used();
-      assert Inodes_all_Valid(inodes);
-      ghost var this_ino := ino;
-      forall ino | ino_ok(ino)
-        ensures inode_blks_match(inodes[ino], inode_blks[ino], data_block)
-      {
-        inode_blks_match_change_other(ino, old(inode_blks[ino]),
-          old(inodes), old(data_block), old(block_used),
-          this_ino, bn, blk.data);
-      }
 
       assert Valid_jrnl_to_all() by {
         reveal_Valid_jrnl_to_block_used();
@@ -445,7 +326,6 @@ module Fs {
       requires is_inode(ino, i)
       ensures Valid()
       ensures is_cur_inode(ino, i)
-      ensures inode_blks == old(inode_blks)
       ensures inodes == old(inodes)
       ensures block_used == old(block_used)
       ensures data_block == old(data_block)
@@ -462,8 +342,9 @@ module Fs {
       requires txn.jrnl == this.jrnl
       requires is_inode(ino, i)
       ensures ValidQ()
-      ensures inode_blks == old(inode_blks)
       ensures inodes == old(inodes)
+      ensures data_block == old(data_block)
+      ensures block_used == old(block_used)
     {
       cur_inode := None;
       inode_inbounds(jrnl, ino);
@@ -490,7 +371,21 @@ module Fs {
       }
     }
 
-    // private
+    // public
+    method getInode(txn: Txn, ino: Ino) returns (i:Inode.Inode)
+      modifies {}
+      requires ValidQ()
+      requires ino_ok(ino)
+      requires txn.jrnl == jrnl
+      ensures is_inode(ino, i)
+    {
+      reveal_Valid_jrnl_to_inodes();
+      inode_inbounds(jrnl, ino);
+      var buf := txn.Read(InodeAddr(ino), 128*8);
+      i := Inode.decode_ino(buf, inodes[ino]);
+    }
+
+    // public
     ghost method writeInode(ino: Ino, i': Inode.Inode)
       modifies this, jrnl
       requires Valid_jrnl_to_all() ensures Valid_jrnl_to_all()
@@ -501,7 +396,6 @@ module Fs {
       ensures inodes == old(inodes)[ino:=i']
       ensures block_used == old(block_used)
       ensures data_block == old(data_block)
-      ensures inode_blks == old(inode_blks)
     {
       inodes := inodes[ino:=i'];
 
@@ -510,65 +404,6 @@ module Fs {
         reveal_Valid_jrnl_to_data_block();
         reveal_Valid_jrnl_to_inodes();
       }
-    }
-
-    // public
-    ghost method writeInodeSz(ino: Ino, i: Inode.Inode, i': Inode.Inode)
-      modifies this, jrnl
-      requires Valid() ensures Valid()
-      requires is_cur_inode(ino, i)
-      requires i'.blks == i.blks
-      requires i'.Valid()
-      ensures is_cur_inode(ino, i')
-      ensures
-      && inodes == old(inodes)[ino:=i']
-      && block_used == old(block_used)
-      && data_block == old(data_block)
-      && inode_blks == old(inode_blks[ino:=inode_blks[ino].(sz := i'.sz as nat)])
-    {
-      writeInode(ino, i');
-      inode_blks := inode_blks[ino:=inode_blks[ino].(sz := i'.sz as nat)];
-      assert Valid() by {
-        reveal_Valid_inodes_to_block_used();
-        reveal_Valid_jrnl_to_inodes();
-      }
-    }
-
-    static lemma inode_blks_match_change_1(
-      i: Inode.Inode, d: InodeData, data_block: map<Blkno, Block>,
-      i': Inode.Inode, bn: Blkno, blkoff: nat, bs: seq<byte>)
-      requires inode_blks_match(i, d, data_block)
-      requires blkoff < |i.blks|
-      requires |bs| == 4096
-      requires i.Valid()
-      requires i'.Valid()
-      requires i'.blks == i.blks
-      requires bn in data_block
-      requires bn != 0
-      requires i.blks[blkoff] == bn
-      ensures inode_blks_match(i', InodeData(i'.sz as nat, d.blks[blkoff:=bs]), data_block[bn := bs])
-    {
-      Inode.reveal_blks_unique();
-      reveal_blks_match?();
-    }
-
-    // inode_blks_match is insensitive to changes in blocks owned by other inodes
-    static lemma inode_blks_match_change_other(
-      ino: Ino, d: InodeData,
-      inodes: map<Ino, Inode.Inode>,
-      data_block: map<Blkno, Block>,
-      block_used: map<Blkno, Option<Ino>>,
-      // stuff that changed in an unrelated inode ino':
-      ino': Ino, bn: Blkno, bs: Block)
-      requires && blkno_dom(data_block) && blkno_dom(block_used) && blkno_ok(bn)
-      requires && ino_dom(inodes) && ino_ok(ino) && ino_ok(ino')
-      requires inode_blks_match(inodes[ino], d, data_block)
-      requires Valid_inodes_to_block_used(inodes, block_used)
-      requires block_used[bn] == Some(ino')
-      ensures ino != ino' ==> inode_blks_match(inodes[ino], d, data_block[bn:=bs])
-    {
-      reveal_Valid_inodes_to_block_used();
-      reveal_blks_match?();
     }
 
     predicate is_inode(ino: Ino, i: Inode.Inode)
@@ -590,32 +425,16 @@ module Fs {
     }
 
     // public
-    method getInode(txn: Txn, ino: Ino) returns (i:Inode.Inode)
-      modifies {}
-      requires ValidQ()
-      requires ino_ok(ino)
-      requires txn.jrnl == jrnl
-      ensures is_inode(ino, i)
-    {
-      reveal_Valid_jrnl_to_inodes();
-      inode_inbounds(jrnl, ino);
-      var buf := txn.Read(InodeAddr(ino), 128*8);
-      i := Inode.decode_ino(buf, inodes[ino]);
-    }
-
-    // private
-    method allocateTo(txn: Txn, ghost ino: Ino, ghost i: Inode.Inode) returns (ok: bool, bn:Blkno)
+    method allocateTo(txn: Txn, ghost state: AllocState)
+      returns (ok: bool, bn:Blkno)
       modifies Repr()
       requires Valid() ensures Valid()
       requires txn.jrnl == jrnl
-      requires is_inode(ino, i)
-      ensures inode_blks == old(inode_blks)
       ensures inodes == old(inodes)
       ensures cur_inode == old(cur_inode)
       ensures data_block == old(data_block)
       ensures !ok ==> block_used == old(block_used)
-      ensures ok ==> forall ino | ino_ok(ino) :: bn !in inodes[ino].blks
-      ensures ok ==> block_used == old(block_used[bn:=Some(ino)])
+      ensures ok ==> block_used == old(block_used[bn:=Some(state)])
       ensures ok ==> is_alloc_bn(bn)
       ensures ok ==> old(block_used[bn].None?)
     {
@@ -623,10 +442,9 @@ module Fs {
       if !ok {
         return;
       }
-      free_block_unused(bn);
 
       blkno_bit_inbounds(jrnl);
-      block_used := block_used[bn:=Some(ino)];
+      block_used := block_used[bn:=Some(state)];
       txn.WriteBit(DataBitAddr(bn), true);
 
       assert Valid_jrnl_to_all() by {
@@ -636,138 +454,29 @@ module Fs {
         DataBitAddr_disjoint(bn);
       }
 
-      reveal_Valid_inodes_to_block_used();
-
       return;
     }
 
-    // private
-    // TODO: not used yet to reclaim blocks
-    method zeroFrom(txn: Txn, ghost ino: Ino, i: Inode.Inode, blkoff: nat)
-      returns (i': Inode.Inode)
+    method free(txn: Txn, bn: Blkno)
       modifies Repr()
       requires Valid() ensures Valid()
       requires txn.jrnl == jrnl
-      requires is_cur_inode(ino, i)
-      requires |i.blks|-1 >= i.used_blocks
-      requires blkoff < 15
-      ensures is_cur_inode(ino, i')
-      ensures i' == i.(blks := i.blks[blkoff := 0])
-      ensures (
-      var d0 := old(inode_blks[ino]);
-      var d' := d0.(blks := d0.blks[blkoff := block0]);
-      inode_blks == old(inode_blks[ino:=d'])
-      )
+      requires blkno_ok(bn)
+      requires block_used[bn].Some?
+      ensures inodes == old(inodes)
+      ensures block_used == old(block_used[bn:=None])
+      ensures cur_inode == old(cur_inode)
+      ensures data_block == old(data_block)
     {
-      var bn := i.blks[blkoff];
-      if bn == 0 {
-        i' := i;
-        ghost var d0 := inode_blks[ino];
-        assert d0.blks[blkoff] == block0 by {
-          reveal_blks_match?();
-        }
-        assert d0.(blks := d0.blks[blkoff := block0]) == d0;
-        return;
-      }
-
-      assert blkno_ok(bn) by {
-        reveal_blks_match?();
-      }
-
-      balloc.Free(bn);
-
       blkno_bit_inbounds(jrnl);
+      block_used := block_used[bn:=None];
       txn.WriteBit(DataBitAddr(bn), false);
-      block_used := block_used[bn := None];
 
       assert Valid_jrnl_to_all() by {
         reveal_Valid_jrnl_to_block_used();
-        reveal_Valid_jrnl_to_inodes();
         reveal_Valid_jrnl_to_data_block();
-      }
-
-      i' := i.(blks := i.blks[blkoff := 0]);
-      assert i'.Valid() by {
-        // TODO: use this syntax everywhere
-        reveal Inode.blks_unique();
-      }
-
-      writeInode(ino, i');
-
-      ghost var d0 := inode_blks[ino];
-      inode_blks := inode_blks[ino := d0.(blks := d0.blks[blkoff := block0])];
-
-      assert Valid_jrnl_to_all() by {
-        reveal_Valid_jrnl_to_block_used();
         reveal_Valid_jrnl_to_inodes();
-        reveal_Valid_jrnl_to_data_block();
-      }
-
-      assert Valid_data() by {
-        reveal_blks_match?();
-      }
-
-      assert Valid_inodes() by {
-        reveal_Valid_inodes_to_block_used();
-        Inode.reveal_blks_unique();
-        forall bn | bn in inodes[ino].blks && bn != 0
-          ensures blkno_ok(bn)
-          ensures block_used[bn] == Some(ino)
-        {
-          assert bn in old(inodes[ino].blks);
-        }
-      }
-    }
-
-    // public
-    method allocateToInode(txn: Txn, ghost ino: Ino, i: Inode.Inode, blkoff: nat)
-      returns (ok: bool, i': Inode.Inode, bn: Blkno)
-      modifies Repr()
-      requires Valid() ensures Valid()
-      requires txn.jrnl == jrnl
-      requires is_cur_inode(ino, i) ensures is_cur_inode(ino, i')
-      requires blkoff < 15 && i.blks[blkoff] == 0
-      // guarantees bn != 0
-      ensures ok ==> is_alloc_bn(bn)
-      ensures ok ==> inode_blks ==
-        old(var d0 := inode_blks[ino];
-            var d' := d0.(blks := d0.blks[blkoff:= data_block[bn]]);
-            inode_blks[ino := d'])
-      ensures !ok ==> inode_blks == old(inode_blks)
-      ensures ok ==> i' == i.(blks := i.blks[blkoff := bn])
-      ensures ok ==> old(block_used[bn].None?)
-    {
-      ok, bn := allocateTo(txn, ino, i);
-      if !ok {
-        i' := i;
-        return;
-      }
-      ok := true;
-
-      // this is the garbage data we're adding to the inode
-      ghost var data := data_block[bn];
-
-      i' := i.(blks := i.blks[blkoff := bn]);
-      assert i'.Valid() by {
-        Inode.blks_unique_extend(i.blks, blkoff, bn);
-      }
-      writeInode(ino, i');
-
-      ghost var d0 := inode_blks[ino];
-      ghost var d' := d0.(blks := d0.blks[blkoff := data]);
-      inode_blks := inode_blks[ino := d'];
-
-      assert inode_blks_match(i', d', data_block) by {
-        reveal_blks_match?();
-      }
-
-      assert Valid_jrnl_to_all() by {
-        reveal Valid_jrnl_to_inodes();
-        reveal Valid_jrnl_to_block_used();
-      }
-
-      assert Valid() by {
-        reveal Valid_inodes_to_block_used();
+        DataBitAddr_disjoint(bn);
       }
     }
 
@@ -783,55 +492,5 @@ module Fs {
       sz := i.sz;
       var _ := txn.Commit();
     }
-
-    // public
-    method getInodeBlk(txn: Txn, ghost ino: Ino, i: Inode.Inode, blkoff: nat)
-      returns (bs: Bytes)
-      modifies {}
-      requires Valid() ensures Valid()
-      requires
-      && this.jrnl == txn.jrnl
-      && is_inode(ino, i)
-      requires blkoff < 15
-      ensures fresh(bs)
-      ensures
-      && is_block(bs.data)
-      && bs.data == inode_blks[ino].blks[blkoff]
-      // && blkno_ok(i.blks[blkoff])
-      // && block_used[i.blks[blkoff]] == Some(ino)
-    {
-      var bn := i.blks[blkoff];
-      reveal_blks_match?();
-      if bn == 0 {
-        bs := NewBytes(4096);
-        return;
-      }
-      datablk_inbounds(jrnl, bn);
-      bs := txn.Read(DataBlk(bn), 4096*8);
-      reveal_Valid_inodes_to_block_used();
-      reveal_Valid_jrnl_to_data_block();
-    }
-
-    lemma inode_sz_no_overflow(ino: Ino, i: Inode.Inode, delta: uint64)
-      requires Valid()
-      requires is_inode(ino, i)
-      requires delta as nat <= 8192
-      ensures no_overflow(i.sz as nat, delta as nat)
-    {}
-
-    // public
-    // TODO: change this to zero a specified tail of the file
-    method freeUnused(txn: Txn, ino: Ino, i: Inode.Inode) returns (i': Inode.Inode)
-      modifies Repr()
-      requires Valid()
-      requires txn.jrnl == jrnl
-      requires is_cur_inode(ino, i)
-      ensures Valid()
-      ensures is_cur_inode(ino, i')
-      ensures inode_blks == old(inode_blks)
-    {
-      i' := i;
-    }
-
   }
 }
